fairness/examples/ticketlock/ext_models.v
@@ -1,0 +1,69 @@
+From trillium.fairness Require Import fairness fair_termination.
+From trillium.fairness.examples.ticketlock Require Import set_map_properties.
+
+(* TODO: can it be generalized to Model? *)
+Section ExtModels.
+  Context (M: FairModel).
+  
+  Context {EI: Type}. (* indexes over external transitions *)
+  Context {DecEI: EqDecision EI} {CntEI: Countable EI}.
+  Context (ETs: EI -> relation (fmstate M)). 
+
+  (* Ensures that in any state there is only a finite amount 
+     of possible external transitions, even if EI is infinite *)
+  Context (active_exts: fmstate M -> gset EI). 
+  Hypothesis (active_exts_spec: forall st ι, ι ∈ active_exts st <-> ∃ st', ETs ι st st').
+
+
+  Inductive env_role := env (i: EI).
+  Definition ext_role: Type := (fmrole M + env_role). 
+
+  Global Instance env_role_EqDec: EqDecision env_role. 
+  Proof using -DecEI. clear -DecEI. solve_decision. Qed. 
+
+  Global Instance env_role_cnt: Countable env_role. 
+  Proof.
+    refine {| 
+        encode r := match r with | env i => encode i end;
+        decode i := match (decode i) with | Some r => Some (env r) | None => None end
+      |}.
+    intros. destruct x.
+    by rewrite decode_encode.
+  Qed.
+
+  Inductive ext_trans: fmstate M -> option ext_role -> fmstate M -> Prop :=
+  | ext_model_step s1 ρ s2 (STEP: fmtrans M s1 (Some ρ) s2):
+    ext_trans s1 (Some (inl ρ)) s2
+  | ext_ext_step s1 s2 ι (REL: ETs ι s1 s2):
+    ext_trans s1 (Some (inr (env ι))) s2. 
+
+  Definition ext_live_roles (st: fmstate M): gset ext_role :=
+    set_map inl (live_roles M st) ∪
+    set_map (inr ∘ env) (active_exts st). 
+
+  Lemma ext_live_spec:
+    ∀ s ρ s', ext_trans s (Some ρ) s' → ρ ∈ ext_live_roles s.
+  Proof using.
+    intros s ρ s' TRANS. unfold ext_live_roles.
+    inversion TRANS; subst; simpl in *.
+    - apply elem_of_union_l. apply elem_of_map_2. 
+      eapply fm_live_spec; eauto. 
+    - apply elem_of_union_r.
+      rewrite set_map_compose_gset. 
+      do 2 apply elem_of_map_2.
+      apply active_exts_spec. eauto.
+  Qed.
+  
+  Definition ext_model: FairModel.
+  Proof using All. 
+    refine({|
+              fmstate := fmstate M;
+              fmrole := ext_role;
+              fmtrans := ext_trans;
+              live_roles := ext_live_roles;
+              fm_live_spec := ext_live_spec
+            |}).
+    apply M. 
+  Defined.
+
+End ExtModels. 
