fairness/examples/ticketlock/trace_helpers.v
@@ -1,0 +1,197 @@
+From iris.proofmode Require Import tactics.
+From hahn Require Import HahnBase.
+From trillium.fairness.examples.ticketlock Require Import lemmas trace_len set_map_properties.
+
+
+(* TODO: inherited from hahn? *)
+Close Scope Z_scope. 
+
+Section TraceHelpers.
+  Context {St L: Type}.
+
+  Lemma pred_at_dec (P: St → option L → Prop)
+    (DEC: forall st ro, Decision (P st ro)):
+    forall tr i, Decision (pred_at tr i P).
+  Proof using.
+    intros tr i. unfold pred_at.
+    destruct (after i tr); [destruct t| ]; auto.
+    solve_decision.
+  Qed.
+
+End TraceHelpers. 
+
+Section FMTraceHelpers.
+  Context {M: FairModel}.
+  Let St := fmstate M.
+  Let L := fmrole M.
+  
+  Definition set_fair_model_trace (T: L -> Prop) tr :=
+    forall ρ (Tρ: T ρ), fair_model_trace ρ tr. 
+
+  (* TODO: already exists somewhere? *)
+  Lemma Decision_iff_impl (P Q: Prop) (PQ: P <-> Q) (DEC_P: Decision P):
+    Decision Q. 
+  Proof using. 
+    destruct DEC_P; [left | right]; tauto. 
+  Qed.
+
+  Lemma pred_at_or P1 P2 (tr: mtrace M) i: 
+    pred_at tr i P1 \/ pred_at tr i P2 <-> pred_at tr i (fun x y => P1 x y \/ P2 x y).
+  Proof using.
+    unfold pred_at. destruct (after i tr); [destruct t| ]; tauto.
+  Qed.
+  
+
+  Definition strong_fair_model_trace (tr: mtrace M) (ρ: fmrole M) :=
+    forall n (EN: pred_at tr n (λ δ _, role_enabled_model ρ δ)),
+    exists m, ClassicalFacts.Minimal 
+                (fun x => pred_at tr (n+x) (λ δ ℓ, ¬ role_enabled_model ρ δ \/ 
+                                                     ℓ = Some (Some ρ))) m.
+
+
+  Lemma fair_model_trace_defs_equiv (tr: mtrace M) (ρ: fmrole M):
+    fair_model_trace ρ tr <-> strong_fair_model_trace tr ρ.
+  Proof using. 
+    split.
+    2: { intros FAIR. red. intros.
+         red in FAIR. specialize (FAIR n H) as [m [FAIR MIN]].
+         exists m. by apply pred_at_or. }
+
+    intros FAIR. red. intros.
+    red in FAIR.
+    specialize (@FAIR n). destruct FAIR; auto.
+
+    pattern x in H. eapply min_prop_dec in H as [d MIN].
+    { clear x. exists d. 
+      eapply Minimal_proper; eauto. 
+      red. intros. symmetry. apply pred_at_or. }
+
+    intros. eapply Decision_iff_impl. 
+    { symmetry. apply pred_at_or. }
+    eapply pred_at_dec. intros.
+    apply or_dec.
+    2: { solve_decision. }
+    apply not_dec.
+    rewrite /role_enabled_model. solve_decision.
+  Qed. 
+  
+  Definition strong_fair_model_trace_alt (tr: mtrace M) (ρ: fmrole M) :=
+    forall n st (NTH: tr S!! n = Some st) (EN: role_enabled_model ρ st),
+    exists m, ClassicalFacts.Minimal (
+             fun x => (exists st', tr S!! (n + x) = Some st' /\ 
+                             ¬ role_enabled_model ρ st') \/
+                     (tr L!! (n + x) = Some (Some ρ))
+           ) m. 
+
+  Lemma strong_fair_model_trace_alt_defs_equiv (tr: mtrace M) (ρ: fmrole M):
+    strong_fair_model_trace tr ρ <-> strong_fair_model_trace_alt tr ρ.
+  Proof using. 
+    rewrite /strong_fair_model_trace /strong_fair_model_trace_alt. 
+    pose proof trace_has_len tr as [len LEN]. 
+    split; intros. 
+    - specialize (H n). specialize_full H. 
+      { apply pred_at_trace_lookup. eauto. }
+      destruct H as [m [PROP MIN]]. exists m. split.
+      { apply pred_at_or in PROP as [PROP | PROP];
+          [left | right]; apply pred_at_trace_lookup in PROP; desc; eauto. }
+      intros. apply MIN. apply pred_at_trace_lookup.
+      destruct H as [DIS | STEP].
+      { desc. exists st'. eauto. }
+      forward eapply (proj1 (label_lookup_states tr (n + k))) as [[st' ST'] _]; eauto.
+    - apply pred_at_trace_lookup in EN. desc. 
+      specialize (H _ _ EN EN0). desc. destruct H as [PROP MIN].  
+      exists m. split.
+      + apply pred_at_trace_lookup. destruct PROP as [DIS | STEP]; desc; eauto.
+        forward eapply (proj1 (label_lookup_states tr (n + m))) as [[st' ST'] _]; eauto.
+      + intros. apply MIN. apply pred_at_or in H. destruct H as [DIS | STEP].
+        * left. apply pred_at_trace_lookup in DIS. eauto. 
+        * right. apply pred_at_trace_lookup in STEP. desc. eauto. 
+  Qed.        
+  
+  Section ValidTracesProperties.
+    Context {tr: mtrace M} (VALID: mtrace_valid tr). 
+
+    From Paco Require Import pacotac.
+    Local Ltac gd t := generalize dependent t.
+
+    Lemma mtrace_valid_steps' i st ℓ st'
+      (ITH: tr !! i = Some (st, Some (ℓ, st'))):
+      fmtrans _ st ℓ st'. 
+    Proof using VALID.
+      gd st. gd ℓ. gd st'. gd tr. clear dependent tr. 
+      induction i. 
+      { simpl. intros. punfold VALID. inversion VALID.
+        - subst. done.
+        - subst. inversion ITH. by subst. }
+      intros. simpl in ITH.
+      destruct tr.
+      { inversion ITH. }
+      punfold VALID. inversion_clear VALID; pclearbot; auto.
+      eapply IHi; eauto. 
+    Qed.
+    
+    Definition label_kept_state (P: St -> Prop) (ℓ: L) :=
+      forall st oℓ' st' (Ps: P st) (OTHER: oℓ' ≠ Some ℓ) (STEP: fmtrans _ st oℓ' st'), 
+        P st'.
+    
+    Lemma steps_keep_state i (P: St -> Prop) ℓ j
+      (Pi: exists st, tr S!! i = Some st /\ P st)    
+      (P_KEPT: label_kept_state P ℓ)
+      (NOρ: forall (k: nat) oℓ' (IKJ: i <= k < j), tr L!! k = Some oℓ' -> oℓ' ≠ Some ℓ):
+      forall k st' (IKJ: i <= k <= j) (KTH: tr S!! k = Some st'), P st'.
+    Proof using VALID. 
+      intros k st' [IK KJ]. apply Nat.le_sum in IK as [d ->]. gd st'. induction d.
+      { rewrite Nat.add_0_r. destruct Pi as (? & ? & ?). intros. congruence. }
+      intros st'' KTH. rewrite Nat.add_succ_r -Nat.add_1_r in KTH. 
+      pose proof (trace_has_len tr) as [len LEN]. 
+      forward eapply (proj2 (trace_lookup_dom_strong  _ _ LEN (i + d))) as [st' CUR].
+      { eapply state_lookup_dom; eauto. }
+      destruct CUR as (oℓ' & st''_ & (PREV & CUR & STEP)%state_label_lookup).
+      assert (st''_ = st'') as -> by congruence.
+      red in P_KEPT. eapply P_KEPT.
+      - apply IHd; [lia| eauto].
+      - eapply NOρ; eauto. lia.
+      - eapply mtrace_valid_steps'; eauto. 
+        apply state_label_lookup. eauto. 
+    Qed.
+    
+    (* TODO: rename *)
+    Lemma kept_state_fair_step (ρ: L) (P: St -> Prop)
+      (KEPT: label_kept_state P ρ)
+      (P_EN: forall st (Pst: P st), @role_enabled_model M ρ st)
+      (FAIRρ: fair_model_trace ρ tr):
+      forall i st (ITH: tr S!! i = Some st) (Pst: P st),
+      exists j st', ClassicalFacts.Minimal (fun j => i <= j /\ tr L!! j = Some $ Some ρ) j /\
+                 tr S!! j = Some st' /\ P st'.
+    Proof using VALID.
+      intros. 
+      apply fair_model_trace_defs_equiv, strong_fair_model_trace_alt_defs_equiv in FAIRρ.         
+      red in FAIRρ. edestruct FAIRρ as [d [STEP MIN]]; [eauto| ..].
+      { apply P_EN. eauto. }
+      clear FAIRρ. 
+
+      pose proof (trace_has_len tr) as [len LEN].
+      assert (my_omega.NOmega.lt_nat_l (i + d) len) as DOMid.
+      { destruct STEP; desc.
+        - eapply state_lookup_dom; eauto.
+        - apply my_omega.NOmega.lt_lt_nat with (m := i + d + 1); [lia| ].
+          eapply label_lookup_dom; eauto. }
+      pose proof (proj2 (state_lookup_dom _ _ LEN (i + d)) DOMid) as [st' IDTH].
+      
+      forward eapply steps_keep_state with (i := i) (j := i + d) (k := i + d) as NEXT_EN; eauto. 
+      { intros. destruct IKJ as [[v ->]%Nat.le_sum KJ]. 
+        intros ->. enough (d <= v); [lia| ]. apply MIN. eauto. }
+      { lia. }
+      
+      destruct STEP as [(st'_ & ST' & DIS') | STEP].
+      { assert (st'_ = st') as -> by congruence. 
+        destruct DIS'. apply P_EN. eauto. }
+      exists (i + d), st'. split; eauto.
+      red. split; [split; [lia| eauto]| ].
+      intros k [LE' STEP']. apply Nat.le_sum in LE' as [d' ->].
+      enough (d <= d'); [lia| ]. apply MIN. eauto.
+    Qed.
+
+  End ValidTracesProperties.
+
+End FMTraceHelpers.
